Source/DafnyCompilers/Interp.dfy
@@ -5,34 +5,39 @@ include "Values.dfy"
 module Interp {
   import Lib.Math
   import Lib.Debug
-  import opened Lib.Datatypes
-  import opened DafnyCompilerCommon.AST
-  import opened DafnyCompilerCommon.Predicates
-  import V = Values
+  import Lib.Seq
 
-  predicate method Pure1(e: Expr) {
+  import V = Values
+  import DafnyCompilerCommon.AST.Types
+  import DafnyCompilerCommon.AST.Exprs
+
+  import opened Lib.Datatypes
+  import opened DafnyCompilerCommon.Predicates
+
+  // FIXME move
+  predicate method Pure1(e: Exprs.T) {
     match e {
       case Var(_) => true
       case Literal(lit) => true
       case Abs(vars, body) => true
-      case Apply(Lazy(op), args: seq<Expr>) =>
+      case Apply(Lazy(op), args) =>
         true
-      case Apply(Eager(op), args: seq<Expr>) =>
+      case Apply(Eager(op), args) =>
         match op {
-          case UnaryOp(uop: UnaryOp.Op) => true
-          case BinaryOp(bop: BinaryOp) => true
-          case TernaryOp(top: TernaryOp) => true
+          case UnaryOp(uop) => true
+          case BinaryOp(bop) => true
+          case TernaryOp(top) => true
           case Builtin(Display(_)) => true
           case Builtin(Print) => false
           case FunctionCall() => true
-          case DataConstructor(name: Path, typeArgs: seq<Type.Type>) => true
+          case DataConstructor(name, typeArgs) => true
         }
-      case Block(stmts: seq<Expr>) => true
-      case If(cond: Expr, thn: Expr, els: Expr) => true
+      case Block(stmts) => true
+      case If(cond, thn, els) => true
     }
   }
 
-  predicate method Pure(e: Expr) {
+  predicate method Pure(e: Exprs.T) {
     Predicates.Deep.All_Expr(e, Pure1)
   }
 
@@ -40,7 +45,7 @@ module Interp {
     match op {
       case UnaryOp(uop) => !uop.MemberSelect?
       case BinaryOp(bop) => !bop.BV? && !bop.Datatypes?
-      case TernaryOp(top: TernaryOp) => true
+      case TernaryOp(top) => true
       case Builtin(Display(_)) => true
       case Builtin(Print()) => false
       case FunctionCall() => true
@@ -48,61 +53,34 @@ module Interp {
     }
   }
 
-  predicate method SupportsInterp1(e: Expr) {
+  predicate method SupportsInterp1(e: Exprs.T) {
     AST.Exprs.WellFormed(e) &&
     match e {
       case Var(_) => true
       case Literal(lit) => true
       case Abs(vars, body) => true
-      case Apply(Lazy(op), args: seq<Expr>) =>
-        true
-      case Apply(Eager(op), args: seq<Expr>) =>
-        EagerOpSupportsInterp(op)
-      case Block(stmts: seq<Expr>) => Debug.TODO(false)
-      case If(cond: Expr, thn: Expr, els: Expr) => true
+      case Apply(Lazy(op), args) => true
+      case Apply(Eager(op), args) => EagerOpSupportsInterp(op)
+      case Block(stmts) => Debug.TODO(false)
+      case If(cond, thn, els) => true
     }
   }
 
   // TODO: I'm not sure it was worth making this opaque.
-  predicate method {:opaque} SupportsInterp(e: Expr) {
+  predicate method {:opaque} SupportsInterp(e: Exprs.T) {
     Predicates.Deep.All_Expr(e, SupportsInterp1)
   }
 
-  lemma SupportsInterp_Pure(e: Expr)
+  lemma SupportsInterp_Pure(e: Exprs.T)
     requires SupportsInterp1(e)
     ensures Pure1(e)
   {}
-
-  // FIXME many "Invalid" below should really be type errors
-
-  datatype InterpError =
-    | OutOfFuel(fn: V.T)
-    | TypeError(e: Expr, value: V.T, expected: Type) // TODO rule out type errors through Wf predicate?
-    | Invalid(e: Expr) // TODO rule out in Wf predicate?
-    | OutOfIntBounds(x: int, low: Option<int>, high: Option<int>)
-    | OutOfSeqBounds(collection: V.T, idx: V.T)
-    | UnboundVariable(v: string)
-    | SignatureMismatch(vars: seq<string>, argvs: seq<V.T>)
-    | DivisionByZero
-  {
-    function method ToString() : string {
-      match this // TODO include values in messages
-        case OutOfFuel(fn) => "Too many function evaluations"
-        case TypeError(e, value, expected) => "Type mismatch"
-        case Invalid(e) => "Invalid expression"
-        case OutOfIntBounds(x, low, high) => "Out-of-bounds value"
-        case OutOfSeqBounds(v, i) => "Out-of-bounds index"
-        case UnboundVariable(v) => "Unbound variable '" + v + "'"
-        case SignatureMismatch(vars, argvs) => "Wrong number of arguments in function call"
-        case DivisionByZero() => "Division by zero"
-    }
-  }
 
   // TODO: rewrite as a shallow predicate applied through ``v.All``?
   predicate method WellFormedEqValue(v: V.T)
   // This predicate gives the constrainst we need to be able to *define* our equivalence relation
   // over values and actually *use* this relation to prove equivalence properties between expressions.
-  // 
+  //
   // The difficult point is linked to closures: when we apply transformations to the code, we often
   // apply them in a deep manner to the expressions (i.e., to all the subexpressions of an expression).
   // The problem is that it can have an effect on the closure values generated through the execution
@@ -181,59 +159,19 @@ module Interp {
     forall v' | v' in ctx.Values :: WellFormedValue(v')
   }
 
-  type Ctx = c: V.Context | WellFormedContext(c)
-
-  datatype State_ =
-    State_(locals: Ctx := map[])
-  {
-    static const Empty: State := State_()
-
-    predicate method WellFormed() {
-      WellFormedContext(this.locals)
-    }
-  }
-
-  type State =
-    s: State_ | s.WellFormed()
-    witness State_()
-
-  datatype InterpReturn_<+A> =
-    | Return(ret: A, ctx: State)
-  {
-    predicate method WellFormed() {
-      this.ctx.WellFormed()
-    }
-  }
-
-  type InterpReturn<+A(0)> = // FIXME: https://github.com/dafny-lang/dafny/issues/2103
-    r: InterpReturn_<A> | r.WellFormed()
-    witness *
-
-  type InterpResult<+A(0)> =
-    Result<InterpReturn<A>, InterpError>
-
-  type PureInterpResult<+A> =
-    Result<A, InterpError>
-
-  function method LiftPureResult<A>(ctx: State, r: PureInterpResult<A>)
-    : InterpResult<A>
-  {
-    var v :- r;
-    Success(Return(v, ctx))
-  }
-
-  // The type of well-formed values manipulated by the interpreter
-  // TODO: rename to ``Value``
-  type WV = v: V.T | WellFormedValue(v) witness V.Bool(false)
+  type Type = Types.T
+  type Context = c: V.Context | WellFormedContext(c)
+  type Value = v: V.T | WellFormedValue(v) witness V.Bool(false)
+  type Expr = e: Exprs.T | SupportsInterp(e) witness (reveal SupportsInterp(); Exprs.Literal(Exprs.LitInt(0)))
 
   // The type of well-formed values with a decidable equality
   type EqWV = v: V.T | WellFormedValue(v) && HasEqValue(v) witness V.Bool(false)
 
   // We need a value type height to prove that some functions terminate.
-  function {:axiom} ValueTypeHeight(v: WV): nat
+  function {:axiom} ValueTypeHeight(v: Value): nat
 
   // Axiom: the children of a collection have a smaller type than the collection's type
-  lemma {:axiom} ValueTypeHeight_Children_Lem(v: WV)
+  lemma {:axiom} ValueTypeHeight_Children_Lem(v: Value)
     requires v.Map? || v.Multiset? || v.Seq? || v.Set?
     ensures forall x | x in v.Children() :: ValueTypeHeight(x) < ValueTypeHeight(v)
     // Special case for the keys of a map
@@ -253,17 +191,66 @@ module Interp {
     }
   }
 
-  function method {:opaque} InterpExpr(e: Expr, fuel: nat, ctx: State := State.Empty)
-    : (r: InterpResult<WV>)
+  datatype State =
+    State(locals: Context := map[])
+  {
+    static const Empty := State(map[]) // BUG(https://github.com/dafny-lang/dafny/issues/2120)
+  }
+
+  datatype Environment =
+    Environment(fuel: nat, globals: Context := map[])
+
+  datatype InterpReturn<+A> =
+    | Return(ret: A, ctx: State)
+
+  // FIXME many "Invalid" below should really be type errors
+
+  datatype InterpError =
+    | OutOfFuel(fn: Value)
+    | TypeError(e: Expr, value: Value, expected: Type) // TODO rule out type errors through Wf predicate?
+    | Invalid(e: Expr) // TODO rule out in Wf predicate?
+    | OutOfIntBounds(x: int, low: Option<int>, high: Option<int>)
+    | OutOfSeqBounds(collection: Value, idx: Value)
+    | UnboundVariable(v: string)
+    | SignatureMismatch(vars: seq<string>, argvs: seq<Value>)
+    | DivisionByZero
+  {
+    function method ToString() : string {
+      match this // TODO include values in messages
+        case OutOfFuel(fn) => "Too many function evaluations"
+        case TypeError(e, value, expected) => "Type mismatch"
+        case Invalid(e) => "Invalid expression"
+        case OutOfIntBounds(x, low, high) => "Out-of-bounds value"
+        case OutOfSeqBounds(v, i) => "Out-of-bounds index"
+        case UnboundVariable(v) => "Unbound variable '" + v + "'"
+        case SignatureMismatch(vars, argvs) => "Wrong number of arguments in function call"
+        case DivisionByZero() => "Division by zero"
+    }
+  }
+
+  type InterpResult<+A> =
+    Result<InterpReturn<A>, InterpError>
+
+  type PureInterpResult<+A> =
+    Result<A, InterpError>
+
+  function method LiftPureResult<A>(ctx: State, r: PureInterpResult<A>)
+    : InterpResult<A>
+  {
+    var v :- r;
+    Success(Return(v, ctx))
+  }
+
+  function method InterpExpr(e: Expr, env: Environment, ctx: State := State.Empty)
+    : (r: InterpResult<Value>)
     requires SupportsInterp(e)
-    decreases fuel, e, 1
+    decreases env.fuel, e, 1
   {
     reveal SupportsInterp();
     Predicates.Deep.AllImpliesChildren(e, SupportsInterp1);
     match e {
       case Var(v) =>
-        var val :- TryGetLocal(ctx, v, UnboundVariable(v));
-        Success(Return(val, ctx))
+        LiftPureResult(ctx, InterpVar(v, ctx, env))
       case Abs(vars, body) =>
         var cv: V.T := V.Closure(ctx.locals, vars, body);
         assert WellFormedValue(cv); // TODO: prove
@@ -271,9 +258,9 @@ module Interp {
       case Literal(lit) =>
         Success(Return(InterpLiteral(lit), ctx))
       case Apply(Lazy(op), args: seq<Expr>) =>
-        InterpLazy(e, fuel, ctx)
+        InterpLazy(e, env, ctx)
       case Apply(Eager(op), args: seq<Expr>) =>
-        var Return(argvs, ctx) :- InterpExprs(args, fuel, ctx);
+        var Return(argvs, ctx) :- InterpExprs(args, env, ctx);
         LiftPureResult(ctx, match op {
             case UnaryOp(op: UnaryOp) =>
               InterpUnaryOp(e, op, argvs[0])
@@ -285,20 +272,28 @@ module Interp {
             case Builtin(Display(ty)) =>
               InterpDisplay(e, ty.kind, argvs)
             case FunctionCall() =>
-              InterpFunctionCall(e, fuel, argvs[0], argvs[1..])
+              InterpFunctionCall(e, env, argvs[0], argvs[1..])
           })
       case If(cond, thn, els) =>
-        var Return(condv, ctx) :- InterpExprWithType(cond, Type.Bool, fuel, ctx);
-        if condv.b then InterpExpr(thn, fuel, ctx) else InterpExpr(els, fuel, ctx)
+        var Return(condv, ctx) :- InterpExprWithType(cond, Type.Bool, env, ctx);
+        if condv.b then InterpExpr(thn, env, ctx) else InterpExpr(els, env, ctx)
     }
   }
 
-  function method {:opaque} TryGetLocal(ctx: State, k: string, err: InterpError)
-    : (r: PureInterpResult<WV>)
-    ensures r.Success? ==> k in ctx.locals && r.value == ctx.locals[k]
-    ensures r.Failure? ==> k !in ctx.locals && r.error == err
+  function method InterpVar(v: string, ctx: State, env: Environment)
+    : PureInterpResult<Value>
   {
-    TryGet(ctx.locals, k, err)
+    match TryGetVariable(ctx.locals, v, UnboundVariable(v))
+      case Success(val) => Success(val)
+      case Failure(err) => TryGetVariable(env.globals, v, err)
+  }
+
+  function method {:opaque} TryGetVariable(ctx: Context, k: string, err: InterpError)
+    : (r: PureInterpResult<Value>)
+    ensures r.Success? ==> k in ctx && r.value == ctx[k]
+    ensures r.Failure? ==> k !in ctx && r.error == err
+  {
+    TryGet(ctx, k, err)
   }
 
   function method {:opaque} TryGet<K, V>(m: map<K, V>, k: K, err: InterpError)
@@ -327,26 +322,26 @@ module Interp {
       MapOfPairs(pairs[..lastidx])[pairs[lastidx].0 := pairs[lastidx].1]
   }
 
-  function method InterpExprWithType(e: Expr, ty: Type, fuel: nat, ctx: State)
-    : (r: InterpResult<WV>)
+  function method InterpExprWithType(e: Expr, ty: Type, env: Environment, ctx: State)
+    : (r: InterpResult<Value>)
     requires SupportsInterp(e)
-    decreases fuel, e, 2
+    decreases env.fuel, e, 2
     ensures r.Success? ==> r.value.ret.HasType(ty)
   {
     reveal SupportsInterp();
-    var Return(val, ctx) :- InterpExpr(e, fuel, ctx);
+    var Return(val, ctx) :- InterpExpr(e, env, ctx);
     :- Need(val.HasType(ty), TypeError(e, val, ty));
     Success(Return(val, ctx))
   }
 
-  function method NeedType(e: Expr, val: WV, ty: Type)
+  function method NeedType(e: Expr, val: Value, ty: Type)
     : (r: Outcome<InterpError>)
     ensures r.Pass? ==> val.HasType(ty)
   {
     Need(val.HasType(ty), TypeError(e, val, ty))
   }
 
-  function method NeedTypes(es: seq<Expr>, vs: seq<WV>, ty: Type)
+  function method NeedTypes(es: seq<Expr>, vs: seq<Value>, ty: Type)
     : (r: Outcome<InterpError>)
     requires |es| == |vs|
     decreases |es|
@@ -369,22 +364,21 @@ module Interp {
         case fail => fail
   }
 
-  // TODO: make opaque?
-  function method {:opaque} InterpExprs(es: seq<Expr>, fuel: nat, ctx: State)
-    : (r: InterpResult<seq<WV>>)
+  function method {:opaque} InterpExprs(es: seq<Expr>, env: Environment, ctx: State)
+    : (r: InterpResult<seq<Value>>)
     requires forall e | e in es :: SupportsInterp(e)
-    decreases fuel, es
+    decreases env.fuel, es
     ensures r.Success? ==> |r.value.ret| == |es|
   { // TODO generalize into a FoldResult function
     reveal SupportsInterp();
     if es == [] then Success(Return([], ctx))
     else
-      var Return(v, ctx) :- InterpExpr(es[0], fuel, ctx);
-      var Return(vs, ctx) :- InterpExprs(es[1..], fuel, ctx);
+      var Return(v, ctx) :- InterpExpr(es[0], env, ctx);
+      var Return(vs, ctx) :- InterpExprs(es[1..], env, ctx);
       Success(Return([v] + vs, ctx))
   }
 
-  function method {:opaque} InterpLiteral(a: AST.Exprs.Literal) : (v: WV)
+  function method {:opaque} InterpLiteral(a: AST.Exprs.Literal) : (v: Value)
     ensures HasEqValue(v)
   {
     match a
@@ -399,36 +393,36 @@ module Interp {
         V.Seq(chars)
   }
 
-  function method {:opaque} InterpLazy(e: Expr, fuel: nat, ctx: State)
-    : (r: InterpResult<WV>)
+  function method {:opaque} InterpLazy(e: Expr, env: Environment, ctx: State)
+    : (r: InterpResult<Value>)
     requires e.Apply? && e.aop.Lazy? && SupportsInterp(e)
-    decreases fuel, e, 0
+    decreases env.fuel, e, 0
   {
     reveal SupportsInterp();
     Predicates.Deep.AllImpliesChildren(e, SupportsInterp1);
     var op, e0, e1 := e.aop.lOp, e.args[0], e.args[1];
-    var Return(v0, ctx0) :- InterpExprWithType(e0, Type.Bool, fuel, ctx);
+    var Return(v0, ctx0) :- InterpExprWithType(e0, Type.Bool, env, ctx);
     match (op, v0)
       case (And, Bool(false)) => Success(Return(V.Bool(false), ctx0))
       case (Or,  Bool(true))  => Success(Return(V.Bool(true), ctx0))
       case (Imp, Bool(false)) => Success(Return(V.Bool(true), ctx0))
       case (_,   Bool(b)) =>
         assert op in {Exprs.And, Exprs.Or, Exprs.Imp};
-        InterpExprWithType(e1, Type.Bool, fuel, ctx0)
+        InterpExprWithType(e1, Type.Bool, env, ctx0)
   }
 
   // Alternate implementation of ``InterpLazy``: less efficient but more closely
   // matching intuition.
-  function method {:opaque} InterpLazy_Eagerly(e: Expr, fuel: nat, ctx: State)
-    : (r: InterpResult<WV>)
+  function method {:opaque} InterpLazy_Eagerly(e: Expr, env: Environment, ctx: State)
+    : (r: InterpResult<Value>)
     requires e.Apply? && e.aop.Lazy? && SupportsInterp(e)
-    decreases fuel, e, 0
+    decreases env.fuel, e, 0
   {
     reveal SupportsInterp();
     Predicates.Deep.AllImpliesChildren(e, SupportsInterp1);
     var op, e0, e1 := e.aop.lOp, e.args[0], e.args[1];
-    var Return(v0, ctx0) :- InterpExprWithType(e0, Type.Bool, fuel, ctx);
-    var Return(v1, ctx1) :- InterpExprWithType(e1, Type.Bool, fuel, ctx0);
+    var Return(v0, ctx0) :- InterpExprWithType(e0, Type.Bool, env, ctx);
+    var Return(v1, ctx1) :- InterpExprWithType(e1, Type.Bool, env, ctx0);
     match (op, v0, v1)
       case (And, Bool(b0), Bool(b1)) =>
         Success(Return(V.Bool(b0 && b1), if b0 then ctx1 else ctx0))
@@ -438,28 +432,28 @@ module Interp {
         Success(Return(V.Bool(b0 ==> b1), if b0 then ctx1 else ctx0))
   }
 
-  lemma InterpLazy_Complete(e: Expr, fuel: nat, ctx: State)
+  lemma InterpLazy_Complete(e: Expr, env: Environment, ctx: State)
     requires e.Apply? && e.aop.Lazy? && SupportsInterp(e)
-    requires InterpLazy(e, fuel, ctx).Failure?
-    ensures InterpLazy_Eagerly(e, fuel, ctx) == InterpLazy(e, fuel, ctx)
+    requires InterpLazy(e, env, ctx).Failure?
+    ensures InterpLazy_Eagerly(e, env, ctx) == InterpLazy(e, env, ctx)
   {
     reveal SupportsInterp();
     reveal InterpLazy();
     reveal InterpLazy_Eagerly();
   }
 
-  lemma InterpLazy_Eagerly_Sound(e: Expr, fuel: nat, ctx: State)
+  lemma InterpLazy_Eagerly_Sound(e: Expr, env: Environment, ctx: State)
     requires e.Apply? && e.aop.Lazy? && SupportsInterp(e)
-    requires InterpLazy_Eagerly(e, fuel, ctx).Success?
-    ensures InterpLazy_Eagerly(e, fuel, ctx) == InterpLazy(e, fuel, ctx)
+    requires InterpLazy_Eagerly(e, env, ctx).Success?
+    ensures InterpLazy_Eagerly(e, env, ctx) == InterpLazy(e, env, ctx)
   {
     reveal SupportsInterp();
     reveal InterpLazy();
     reveal InterpLazy_Eagerly();
   }
 
-  function method {:opaque} InterpUnaryOp(expr: Expr, op: AST.UnaryOp, v0: WV)
-    : (r: PureInterpResult<WV>)
+  function method {:opaque} InterpUnaryOp(expr: Expr, op: AST.UnaryOp, v0: Value)
+    : (r: PureInterpResult<Value>)
     requires !op.MemberSelect?
   {
     match op
@@ -477,8 +471,8 @@ module Interp {
         Success(V.Int(|v0.m|))
   }
 
-  function method {:opaque} InterpBinaryOp(expr: Expr, bop: AST.BinaryOp, v0: WV, v1: WV)
-    : (r: PureInterpResult<WV>)
+  function method {:opaque} InterpBinaryOp(expr: Expr, bop: AST.BinaryOp, v0: Value, v1: Value)
+    : (r: PureInterpResult<Value>)
     requires !bop.BV? && !bop.Datatypes?
   {
     match bop
@@ -500,8 +494,8 @@ module Interp {
       // case Datatypes(op) =>
   }
 
-  function method InterpBinaryNumeric(expr: Expr, op: BinaryOps.Numeric, v0: WV, v1: WV)
-    : (r: PureInterpResult<WV>)
+  function method InterpBinaryNumeric(expr: Expr, op: Exprs.BinaryOps.Numeric, v0: Value, v1: Value)
+    : (r: PureInterpResult<Value>)
   {
     match (v0, v1) {
       // Separate functions to more easily check exhaustiveness
@@ -517,7 +511,7 @@ module Interp {
   }
 
   function method InterpBinaryInt(expr: Expr, bop: AST.BinaryOps.Numeric, x1: int, x2: int)
-    : (r: PureInterpResult<WV>)
+    : (r: PureInterpResult<Value>)
   {
     match bop {
       case Lt() => Success(V.Bool(x1 < x2))
@@ -538,7 +532,7 @@ module Interp {
   }
 
   function method InterpBinaryNumericChar(expr: Expr, bop: AST.BinaryOps.Numeric, x1: char, x2: char)
-    : (r: PureInterpResult<WV>)
+    : (r: PureInterpResult<Value>)
   {
     match bop { // FIXME: These first four cases are not used (see InterpBinaryChar instead)
       case Lt() => Success(V.Bool(x1 < x2))
@@ -554,7 +548,7 @@ module Interp {
   }
 
   function method InterpBinaryReal(expr: Expr, bop: AST.BinaryOps.Numeric, x1: real, x2: real)
-    : (r: PureInterpResult<WV>)
+    : (r: PureInterpResult<Value>)
   {
     match bop {
       case Lt() => Success(V.Bool(x1 < x2))
@@ -569,8 +563,8 @@ module Interp {
     }
   }
 
-  function method InterpBinaryLogical(expr: Expr, op: BinaryOps.Logical, v0: WV, v1: WV)
-    : (r: PureInterpResult<WV>)
+  function method InterpBinaryLogical(expr: Expr, op: Exprs.BinaryOps.Logical, v0: Value, v1: Value)
+    : (r: PureInterpResult<Value>)
   {
     :- Need(v0.Bool? && v1.Bool?, Invalid(expr));
     match op
@@ -578,8 +572,8 @@ module Interp {
         Success(V.Bool(v0.b <==> v1.b))
   }
 
-  function method InterpBinaryChar(expr: Expr, op: AST.BinaryOps.Char, v0: WV, v1: WV)
-    : (r: PureInterpResult<WV>)
+  function method InterpBinaryChar(expr: Expr, op: AST.BinaryOps.Char, v0: Value, v1: Value)
+    : (r: PureInterpResult<Value>)
   { // FIXME eliminate distinction between GtChar and GT?
     :- Need(v0.Char? && v1.Char?, Invalid(expr));
     match op
@@ -593,8 +587,8 @@ module Interp {
         Success(V.Bool(v0.c > v1.c))
   }
 
-  function method InterpBinarySets(expr: Expr, op: BinaryOps.Sets, v0: WV, v1: WV)
-    : (r: PureInterpResult<WV>)
+  function method InterpBinarySets(expr: Expr, op: Exprs.BinaryOps.Sets, v0: Value, v1: Value)
+    : (r: PureInterpResult<Value>)
   {
     // Rk.: we enforce through `WellFormedEqValue` that sets contain values with a decidable
     // equality.
@@ -629,8 +623,8 @@ module Interp {
         Success(V.Bool(v0 !in v1.st))
   }
 
-  function method InterpBinaryMultisets(expr: Expr, op: BinaryOps.Multisets, v0: WV, v1: WV)
-    : (r: PureInterpResult<WV>)
+  function method InterpBinaryMultisets(expr: Expr, op: Exprs.BinaryOps.Multisets, v0: Value, v1: Value)
+    : (r: PureInterpResult<Value>)
   {
     // Rk.: we enforce through `WellFormedEqValue` that multisets contain values with a decidable
     // equality.
@@ -669,8 +663,8 @@ module Interp {
         Success(V.Int(v0.ms[v1]))
   }
 
-  function method InterpBinarySequences(expr: Expr, op: BinaryOps.Sequences, v0: WV, v1: WV)
-    : (r: PureInterpResult<WV>)
+  function method InterpBinarySequences(expr: Expr, op: Exprs.BinaryOps.Sequences, v0: Value, v1: Value)
+    : (r: PureInterpResult<Value>)
   {
     // Rk.: sequences don't necessarily contain values with decidable equality, we
     // thus dynamically check that we have what we need depending on the operation
@@ -721,8 +715,8 @@ module Interp {
         Success(v0.sq[v1.i])
   }
 
-  function method InterpBinaryMaps(expr: Expr, op: BinaryOps.Maps, v0: WV, v1: WV)
-    : (r: PureInterpResult<WV>)
+  function method InterpBinaryMaps(expr: Expr, op: Exprs.BinaryOps.Maps, v0: Value, v1: Value)
+    : (r: PureInterpResult<Value>)
   {
     // Rk.: values in maps don't necessarily have a decidable equality. We thus perform
     // dynamic checks when we need one and fail if it is not the case.
@@ -758,8 +752,8 @@ module Interp {
         Success(v0.m[v1])
   }
 
-  function method {:opaque} InterpTernaryOp(expr: Expr, top: AST.TernaryOp, v0: WV, v1: WV, v2: WV)
-    : (r: PureInterpResult<WV>)
+  function method {:opaque} InterpTernaryOp(expr: Expr, top: AST.TernaryOp, v0: Value, v1: Value, v2: Value)
+    : (r: PureInterpResult<Value>)
   {
     match top
       case Sequences(op) =>
@@ -770,7 +764,7 @@ module Interp {
         InterpTernaryMaps(expr, op, v0, v1, v2)
   }
 
-  function method NeedValidIndex(expr: Expr, vs: WV, vidx: WV)
+  function method NeedValidIndex(expr: Expr, vs: Value, vidx: Value)
     : Outcome<InterpError>
   { // FIXME no monadic operator for combining outcomes?
     match Need(vidx.Int? && vs.Seq?, Invalid(expr))
@@ -778,7 +772,7 @@ module Interp {
       case fail => fail
   }
 
-  function method NeedValidEndpoint(expr: Expr, vs: WV, vidx: WV)
+  function method NeedValidEndpoint(expr: Expr, vs: Value, vidx: Value)
     : Outcome<InterpError>
   {
     match Need(vidx.Int? && vs.Seq?, Invalid(expr))
@@ -786,8 +780,8 @@ module Interp {
       case fail => fail
   }
 
-  function method InterpTernarySequences(expr: Expr, op: AST.TernaryOps.Sequences, v0: WV, v1: WV, v2: WV)
-    : (r: PureInterpResult<WV>)
+  function method InterpTernarySequences(expr: Expr, op: AST.TernaryOps.Sequences, v0: Value, v1: Value, v2: Value)
+    : (r: PureInterpResult<Value>)
   {
     match op
       case SeqUpdate() =>
@@ -800,8 +794,8 @@ module Interp {
         Success(V.Seq(v0.sq[v1.i..v2.i]))
   }
 
-  function method InterpTernaryMultisets(expr: Expr, op: AST.TernaryOps.Multisets, v0: WV, v1: WV, v2: WV)
-    : (r: PureInterpResult<WV>)
+  function method InterpTernaryMultisets(expr: Expr, op: AST.TernaryOps.Multisets, v0: Value, v1: Value, v2: Value)
+    : (r: PureInterpResult<Value>)
   {
     match op
       case MultisetUpdate() =>
@@ -811,8 +805,8 @@ module Interp {
         Success(V.Multiset(v0.ms[v1 := v2.i]))
   }
 
-  function method InterpTernaryMaps(expr: Expr, op: AST.TernaryOps.Maps, v0: WV, v1: WV, v2: WV)
-    : (r: PureInterpResult<WV>)
+  function method InterpTernaryMaps(expr: Expr, op: AST.TernaryOps.Maps, v0: Value, v1: Value, v2: Value)
+    : (r: PureInterpResult<Value>)
   {
     match op
       case MapUpdate() =>
@@ -821,8 +815,8 @@ module Interp {
         Success(V.Map(v0.m[v1 := v2]))
   }
 
-  function method {:opaque} InterpDisplay(e: Expr, kind: Types.CollectionKind, argvs: seq<WV>)
-    : (r: PureInterpResult<WV>)
+  function method {:opaque} InterpDisplay(e: Expr, kind: Types.CollectionKind, argvs: seq<Value>)
+    : (r: PureInterpResult<Value>)
   {
     match kind
       case Map(_) =>
@@ -840,39 +834,46 @@ module Interp {
         Success(V.Set(set s | s in argvs))
   }
 
-  function method InterpMapDisplay(e: Expr, argvs: seq<WV>)
-    : PureInterpResult<map<EqWV, WV>>
+  function method InterpMapDisplay(e: Expr, argvs: seq<Value>)
+    : PureInterpResult<map<EqWV, Value>>
   {
     var pairs :- Seq.MapResult(argvs, argv => PairOfMapDisplaySeq(e, argv));
     Success(MapOfPairs(pairs))
   }
 
-  function method PairOfMapDisplaySeq(e: Expr, argv: WV)
-    : PureInterpResult<(EqWV, WV)>
+  function method PairOfMapDisplaySeq(e: Expr, argv: Value)
+    : PureInterpResult<(EqWV, Value)>
   {
     :- Need(argv.Seq? && |argv.sq| == 2, Invalid(e));
     :- Need(HasEqValue(argv.sq[0]), Invalid(e));
     Success((argv.sq[0], argv.sq[1]))
   }
 
-  function method {:opaque} BuildCallState(captured: Ctx, vars: seq<string>, vals: seq<WV>)
+  function method {:opaque} BuildCallState(captured: Context, vars: seq<string>, vals: seq<Value>)
     : (ctx: State)
     requires |vars| == |vals|
   {
-    State.Empty.(locals := captured + MapOfPairs(Seq.Zip(vars, vals)))
+    State().(locals := captured + MapOfPairs(Seq.Zip(vars, vals)))
   }
 
-  function method {:opaque} InterpFunctionCall(e: Expr, fuel: nat, fn: WV, argvs: seq<WV>)
-    : (r: PureInterpResult<WV>)
-    decreases fuel, e, 0
+  function method {:opaque} BuildCallState(base: Context, vars: seq<string>, vals: seq<Value>)
+    : State
+    requires |vars| == |vals|
   {
-    :- Need(fuel > 0, OutOfFuel(fn));
+    State(locals := AugmentContext(base, vars, vals))
+  }
+
+  function method {:opaque} InterpFunctionCall(e: Expr, env: Environment, fn: Value, argvs: seq<Value>)
+    : (r: PureInterpResult<Value>)
+    decreases env.fuel, e, 0
+  {
+    :- Need(env.fuel > 0, OutOfFuel(fn));
     :- Need(fn.Closure?, Invalid(e));
     reveal SupportsInterp();
     Predicates.Deep.AllImpliesChildren(fn.body, SupportsInterp1);
     :- Need(|fn.vars| == |argvs|, SignatureMismatch(fn.vars, argvs));
     var ctx := BuildCallState(fn.ctx, fn.vars, argvs);
-    var Return(val, ctx) :- InterpExpr(fn.body, fuel - 1, ctx);
+    var Return(val, ctx) :- InterpExpr(fn.body, env.(fuel := env.fuel - 1), ctx);
     Success(val)
   }
 }
